Prove step preserves wf_state
Closes #49

spec/prop/vfmExecutionPropScript.sml
@@ -77,7 +77,7 @@ End
 Definition wf_state_def:
   wf_state s ⇔
     s.contexts ≠ [] ∧
-    LENGTH s.contexts ≤ context_limit ∧
+    LENGTH s.contexts ≤ SUC context_limit ∧
     EVERY wf_context s.contexts ∧
     EVERY wf_accounts (all_accounts s)
 End
@@ -118,29 +118,6 @@ Proof
 QED
 
 (* -- *)
-
-(*
-Definition no_change_to_code_size_def:
-  no_change_to_code_size (a1: evm_accounts) (a2: evm_accounts) =
-  ∀x. 0 < LENGTH (a1 x).code ⇒ LENGTH (a2 x).code = LENGTH (a1 x).code
-End
-
-Theorem no_change_to_code_size_refl[simp]:
-  no_change_to_code_size a a
-Proof
-  rw[no_change_to_code_size_def]
-QED
-
-Theorem no_change_to_code_size_trans[simp]:
-  no_change_to_code_size x y ∧
-  no_change_to_code_size y z ⇒
-  no_change_to_code_size x z
-Proof
-  rw[no_change_to_code_size_def]
-QED
-*)
-
-Theorem no_change_to_code_size_trans[local] = TRUTH;
 
 Definition decreases_gas_def:
   decreases_gas strict (m: α execution) =
@@ -197,7 +174,7 @@ Proof
   \\ Cases_on `s.contexts` \\ rw [] \\ gvs []
   \\ Cases_on `sf` \\ simp []
   \\ rpt (qhdtm_x_assum `COND` mp_tac) \\ rw []
-  \\ metis_tac [no_change_to_code_size_trans]
+  \\ metis_tac []
 QED
 
 Theorem decreases_gas_bind:
@@ -601,7 +578,7 @@ Proof
   \\ last_x_assum (qspecl_then [`y`,`r`] mp_tac) \\ simp []
   \\ Cases_on `s.contexts = []` \\ rpt strip_tac \\ gs []
   \\ qhdtm_x_assum `COND` mp_tac \\ IF_CASES_TAC \\ simp []
-  \\ metis_tac (no_change_to_code_size_trans::lexs)
+  \\ metis_tac (lexs)
 QED
 
 Theorem decreases_gas_cred_true_false:
@@ -631,7 +608,7 @@ Proof
     \\ disch_then (qspec_then `r` mp_tac) \\ fs []
     \\ Cases_on `s.contexts = []` \\ fs []
     \\ qhdtm_x_assum `COND` mp_tac \\ rw []
-    \\ metis_tac (no_change_to_code_size_trans::NOT_ISR_ISL::lexs))
+    \\ metis_tac (NOT_ISR_ISL::lexs))
   \\ Cases_on `s.contexts = []` \\ gs [] \\ metis_tac lexs
 QED
 
@@ -3036,18 +3013,884 @@ Proof
   \\ gs[wf_account_state_def]
 QED
 
+Definition limits_num_contexts_def:
+  limits_num_contexts n1 n2 (m: α execution) =
+  ∀s. LENGTH s.contexts < n1 ⇒
+      LENGTH (SND (m s)).contexts < n2
+End
+
+Theorem limits_num_contexts_bind:
+  (∀x. limits_num_contexts n2 n3 (f x)) ∧
+  limits_num_contexts n1 n2 g ∧
+  n2 ≤ n3
+  ⇒
+  limits_num_contexts n1 n3 (bind g f)
+Proof
+  rw[limits_num_contexts_def, bind_def]
+  \\ CASE_TAC \\ gs[]
+  \\ CASE_TAC \\ gs[]
+  \\ first_x_assum drule \\ rw[]
+QED
+
+Theorem limits_num_contexts_bind_same:
+  (∀x. limits_num_contexts n n (f x)) ∧
+  limits_num_contexts n n g
+  ⇒
+  limits_num_contexts n n (bind g f)
+Proof
+  strip_tac
+  \\ irule limits_num_contexts_bind
+  \\ goal_assum(first_assum o mp_then Any mp_tac)
+  \\ rw[]
+QED
+
 (*
+Theorem limits_num_contexts_bind_pred:
+  (∀x. p x ⇒ limits_num_contexts (f x)) ∧
+  (∀s a. EVERY wf_accounts (all_accounts s) ∧ FST (g s) = (INL a) ⇒ p a) ∧
+  limits_num_contexts g
+  ⇒
+  limits_num_contexts (bind g f)
+Proof
+  rw[limits_num_contexts_def, bind_def]
+  \\ CASE_TAC \\ gs[]
+  \\ CASE_TAC \\ gs[]
+  \\ metis_tac[SND, FST]
+QED
+*)
+
+Theorem limits_num_contexts_ignore_bind:
+  limits_num_contexts n2 n3 f ∧
+  limits_num_contexts n1 n2 g ∧
+  n2 ≤ n3
+  ⇒
+  limits_num_contexts n1 n3 (ignore_bind g f)
+Proof
+  rw[ignore_bind_def]
+  \\ irule limits_num_contexts_bind \\ rw[]
+  \\ goal_assum (first_assum o mp_then Any mp_tac)
+  \\ rw[]
+QED
+
+Theorem limits_num_contexts_ignore_bind_same:
+  limits_num_contexts n n f ∧
+  limits_num_contexts n n g
+  ⇒
+  limits_num_contexts n n (ignore_bind g f)
+Proof
+  strip_tac
+  \\ irule limits_num_contexts_ignore_bind
+  \\ goal_assum(first_assum o mp_then Any mp_tac)
+  \\ rw[]
+QED
+
+Theorem limits_num_contexts_get_current_context[simp]:
+  limits_num_contexts n n get_current_context
+Proof
+  rw[limits_num_contexts_def, get_current_context_def]
+  \\ rw[return_def, fail_def]
+QED
+
+Theorem limits_num_contexts_assert[simp]:
+  limits_num_contexts n n (assert b e)
+Proof
+  rw[limits_num_contexts_def, assert_def]
+QED
+
+Theorem limits_num_contexts_set_current_context[simp]:
+  limits_num_contexts n n (set_current_context c)
+Proof
+  rw[limits_num_contexts_def, set_current_context_def]
+  \\ rw[fail_def, return_def]
+  \\ gs[all_accounts_def]
+  \\ Cases_on`s.contexts` \\ gs[]
+QED
+
+Theorem limits_num_contexts_return[simp]:
+  limits_num_contexts n n (return x)
+Proof
+  rw[return_def, limits_num_contexts_def]
+QED
+
+Theorem limits_num_contexts_fail[simp]:
+  limits_num_contexts n n (fail x)
+Proof
+  rw[fail_def, limits_num_contexts_def]
+QED
+
+val tac = rpt (
+  (irule limits_num_contexts_bind_same \\ rw[]) ORELSE
+  (irule limits_num_contexts_ignore_bind_same \\ rw[])
+)
+
+Theorem limits_num_contexts_pop_stack[simp]:
+  limits_num_contexts n n (pop_stack m)
+Proof
+  rw[pop_stack_def] \\ tac
+QED
+
+Theorem limits_num_contexts_consume_gas[simp]:
+  limits_num_contexts n n (consume_gas m)
+Proof
+  rw[consume_gas_def] \\ tac
+QED
+
+Theorem limits_num_contexts_push_stack[simp]:
+  limits_num_contexts n n (push_stack m)
+Proof
+  rw[push_stack_def] \\ tac
+QED
+
+Theorem limits_num_contexts_step_binop[simp]:
+  limits_num_contexts n n (step_binop x y)
+Proof
+  rw[step_binop_def] \\ tac
+QED
+
+Theorem limits_num_contexts_step_modop[simp]:
+  limits_num_contexts n n (step_modop x y)
+Proof
+  rw[step_modop_def] \\ tac
+QED
+
+Theorem limits_num_contexts_step_monop[simp]:
+  limits_num_contexts n n (step_monop x y)
+Proof
+  rw[step_monop_def] \\ tac
+QED
+
+Theorem limits_num_contexts_get_tx_params[simp]:
+  limits_num_contexts n n get_tx_params
+Proof
+  rw[get_tx_params_def, limits_num_contexts_def, return_def]
+QED
+
+Theorem limits_num_contexts_step_txParams[simp]:
+  limits_num_contexts n n (step_txParams x y)
+Proof
+  rw[step_txParams_def] \\ tac
+QED
+
+Theorem limits_num_contexts_step_context[simp]:
+  limits_num_contexts n n (step_context x y)
+Proof
+  rw[step_context_def] \\ tac
+QED
+
+Theorem limits_num_contexts_step_msgParams[simp]:
+  limits_num_contexts n n (step_msgParams x y)
+Proof
+  rw[step_msgParams_def]
+QED
+
+Theorem limits_num_contexts_memory_expansion_info[simp]:
+  limits_num_contexts n n (memory_expansion_info c e)
+Proof
+  rw[memory_expansion_info_def] \\ tac
+QED
+
+Theorem limits_num_contexts_write_memory[simp]:
+  limits_num_contexts n n (write_memory c e)
+Proof
+  rw[write_memory_def] \\ tac
+QED
+
+Theorem limits_num_contexts_read_memory[simp]:
+  limits_num_contexts n n (read_memory c e)
+Proof
+  rw[read_memory_def] \\ tac
+QED
+
+Theorem limits_num_contexts_expand_memory[simp]:
+  limits_num_contexts n n (expand_memory c)
+Proof
+  rw[expand_memory_def] \\ tac
+QED
+
+Theorem limits_num_contexts_copy_to_memory[simp]:
+  (∀f. e = SOME f ⇒ limits_num_contexts n n f) ⇒
+  limits_num_contexts n n (copy_to_memory a b c d e)
+Proof
+  rw[copy_to_memory_def, max_expansion_range_def]
+  \\ irule limits_num_contexts_bind_same \\ rw[]
+  \\ irule limits_num_contexts_ignore_bind_same \\ rw[]
+  \\ irule limits_num_contexts_bind_same \\ rw[]
+  \\ TRY(irule limits_num_contexts_ignore_bind_same \\ rw[])
+  \\ CASE_TAC \\ gs[]
+  \\ irule limits_num_contexts_bind_same \\ rw[]
+  \\ irule limits_num_contexts_ignore_bind_same \\ rw[]
+QED
+
+Theorem limits_num_contexts_step_copy_to_memory[simp]:
+  (∀f. y = SOME f ⇒ limits_num_contexts n n f) ⇒
+  limits_num_contexts n n (step_copy_to_memory x y)
+Proof
+  rw[step_copy_to_memory_def] \\ tac
+QED
+
+Theorem limits_num_contexts_step_exp[simp]:
+  limits_num_contexts n n step_exp
+Proof
+  rw[step_exp_def] \\ tac
+QED
+
+Theorem limits_num_contexts_step_keccak256[simp]:
+  limits_num_contexts n n step_keccak256
+Proof
+  rw[step_keccak256_def] \\ tac
+QED
+
+Theorem limits_num_contexts_get_accounts[simp]:
+  limits_num_contexts n n get_accounts
+Proof
+  rw[get_accounts_def, limits_num_contexts_def, return_def]
+QED
+
+Theorem limits_num_contexts_access_address[simp]:
+  limits_num_contexts n n (access_address a)
+Proof
+  rw[access_address_def, limits_num_contexts_def, return_def, fail_def]
+  \\ rw[] \\ gs[all_accounts_def]
+QED
+
+Theorem limits_num_contexts_access_slot[simp]:
+  limits_num_contexts n n (access_slot a)
+Proof
+  rw[access_slot_def, limits_num_contexts_def, return_def, fail_def]
+  \\ rw[] \\ gs[all_accounts_def]
+QED
+
+Theorem limits_num_contexts_step_balance[simp]:
+  limits_num_contexts n n step_balance
+Proof
+  rw[step_balance_def] \\ tac
+QED
+
+Theorem limits_num_contexts_get_call_data[simp]:
+  limits_num_contexts n n get_call_data
+Proof
+  rw[get_call_data_def] \\ tac
+QED
+
+Theorem limits_num_contexts_step_call_data_load[simp]:
+  limits_num_contexts n n step_call_data_load
+Proof
+  rw[step_call_data_load_def] \\ tac
+QED
+
+Theorem limits_num_contexts_get_code[simp]:
+  limits_num_contexts n n (get_code x)
+Proof
+  rw[get_code_def] \\ tac
+QED
+
+Theorem limits_num_contexts_get_return_data[simp]:
+  limits_num_contexts n n get_return_data
+Proof
+  rw[get_return_data_def] \\ tac
+QED
+
+Theorem limits_num_contexts_get_return_data_check[simp]:
+  limits_num_contexts n n (get_return_data_check y x)
+Proof
+  rw[get_return_data_check_def] \\ tac
+QED
+
+Theorem limits_num_contexts_step_ext_code_copy[simp]:
+  limits_num_contexts n n step_ext_code_copy
+Proof
+  rw[step_ext_code_copy_def] \\ tac
+QED
+
+Theorem limits_num_contexts_step_ext_code_size[simp]:
+  limits_num_contexts n n step_ext_code_size
+Proof
+  rw[step_ext_code_size_def] \\ tac
+QED
+
+Theorem limits_num_contexts_step_ext_code_hash[simp]:
+  limits_num_contexts n n step_ext_code_hash
+Proof
+  rw[step_ext_code_hash_def] \\ tac
+QED
+
+Theorem limits_num_contexts_step_return_data_copy[simp]:
+  limits_num_contexts n n step_return_data_copy
+Proof
+  rw[step_return_data_copy_def] \\ tac
+QED
+
+Theorem limits_num_contexts_step_block_hash[simp]:
+  limits_num_contexts n n step_block_hash
+Proof
+  rw[step_block_hash_def] \\ tac
+QED
+
+Theorem limits_num_contexts_get_callee[simp]:
+  limits_num_contexts n n get_callee
+Proof
+  rw[get_callee_def] \\ tac
+QED
+
+Theorem limits_num_contexts_step_self_balance[simp]:
+  limits_num_contexts n n step_self_balance
+Proof
+  rw[step_self_balance_def] \\ tac
+QED
+
+Theorem limits_num_contexts_step_pop[simp]:
+  limits_num_contexts n n step_pop
+Proof
+  rw[step_pop_def] \\ tac
+QED
+
+Theorem limits_num_contexts_step_mload[simp]:
+  limits_num_contexts n n step_mload
+Proof
+  rw[step_mload_def] \\ tac
+QED
+
+Theorem limits_num_contexts_step_mstore[simp]:
+  limits_num_contexts n n (step_mstore x)
+Proof
+  rw[step_mstore_def] \\ tac
+QED
+
+Theorem limits_num_contexts_get_tStorage[simp]:
+  limits_num_contexts n n get_tStorage
+Proof
+  rw[get_tStorage_def, limits_num_contexts_def, return_def]
+QED
+
+Theorem limits_num_contexts_step_sload[simp]:
+  limits_num_contexts n n (step_sload x)
+Proof
+  rw[step_sload_def] >> tac
+QED
+
+Theorem limits_num_contexts_get_rollback[simp]:
+  limits_num_contexts n n get_rollback
+Proof
+  rw[get_rollback_def, limits_num_contexts_def, return_def]
+QED
+
+Theorem limits_num_contexts_set_jump_dest[simp]:
+  limits_num_contexts n n (set_jump_dest x)
+Proof
+  rw[set_jump_dest_def] >> tac
+QED
+
+Theorem limits_num_contexts_step_jump[simp]:
+  limits_num_contexts n n step_jump
+Proof
+  rw[step_jump_def] >> tac
+QED
+
+Theorem limits_num_contexts_step_jumpi[simp]:
+  limits_num_contexts n n step_jumpi
+Proof
+  rw[step_jumpi_def] >> tac
+QED
+
+Theorem limits_num_contexts_step_push[simp]:
+  limits_num_contexts n n (step_push x y)
+Proof
+  rw[step_push_def] >> tac
+QED
+
+Theorem limits_num_contexts_step_dup[simp]:
+  limits_num_contexts n n (step_dup x)
+Proof
+  rw[step_dup_def] >> tac
+QED
+
+Theorem limits_num_contexts_step_swap[simp]:
+  limits_num_contexts n n (step_swap x)
+Proof
+  rw[step_swap_def] >> tac
+QED
+
+Theorem limits_num_contexts_push_logs[simp]:
+  limits_num_contexts n n (push_logs x)
+Proof
+  rw[push_logs_def] >> tac
+QED
+
+Theorem limits_num_contexts_get_static[simp]:
+  limits_num_contexts n n get_static
+Proof
+  rw[get_static_def] >> tac
+QED
+
+Theorem limits_num_contexts_assert_not_static[simp]:
+  limits_num_contexts n n assert_not_static
+Proof
+  rw[assert_not_static_def] >> tac
+QED
+
+Theorem limits_num_contexts_step_log[simp]:
+  limits_num_contexts n n (step_log x)
+Proof
+  rw[step_log_def] >> tac
+QED
+
+Theorem limits_num_contexts_set_tStorage[simp]:
+  limits_num_contexts n n (set_tStorage x)
+Proof
+  rw[set_tStorage_def, limits_num_contexts_def, return_def, all_accounts_def]
+QED
+
+Theorem limits_num_contexts_write_transient_storage[simp]:
+  limits_num_contexts n n (write_transient_storage x y z)
+Proof
+  rw[write_transient_storage_def] >> tac
+QED
+
+Theorem limits_num_contexts_write_storage[simp]:
+  limits_num_contexts n n (write_storage x y z)
+Proof
+  rw[write_storage_def] >> tac
+  \\ rw[limits_num_contexts_def, update_accounts_def, return_def]
+QED
+
+Theorem limits_num_contexts_update_gas_refund_def[simp]:
+  limits_num_contexts n n (update_gas_refund x)
+Proof
+  Cases_on`x` >>
+  rw[update_gas_refund_def] >>
+  tac
+QED
+
+Theorem limits_num_contexts_get_original[simp]:
+  limits_num_contexts n n get_original
+Proof
+  rw[get_original_def, limits_num_contexts_def]
+  \\ rw[return_def, fail_def]
+QED
+
+Theorem limits_num_contexts_get_gas_left[simp]:
+  limits_num_contexts n n get_gas_left
+Proof
+  rw[get_gas_left_def] >> tac
+QED
+
+Theorem limits_num_contexts_get_current_code[simp]:
+  limits_num_contexts n n get_current_code
+Proof
+  rw[get_current_code_def] >> tac
+QED
+
+Theorem limits_num_contexts_get_num_contexts[simp]:
+  limits_num_contexts n n get_num_contexts
+Proof
+  rw[get_num_contexts_def, limits_num_contexts_def, return_def]
+QED
+
+Theorem limits_num_contexts_get_value[simp]:
+  limits_num_contexts n n get_value
+Proof
+  rw[get_value_def] >> tac
+QED
+
+Theorem limits_num_contexts_get_caller[simp]:
+  limits_num_contexts n n get_caller
+Proof
+  rw[get_caller_def] >> tac
+QED
+
+Theorem limits_num_contexts_step_sstore_gas_consumption[simp]:
+  limits_num_contexts n n (step_sstore_gas_consumption x y z)
+Proof
+  rw[step_sstore_gas_consumption_def] >> tac
+QED
+
+Theorem limits_num_contexts_step_sstore[simp]:
+  limits_num_contexts n n (step_sstore x)
+Proof
+  rw[step_sstore_def] >> tac
+QED
+
+Theorem limits_num_contexts_finish[simp]:
+  limits_num_contexts n n finish
+Proof
+  rw[finish_def, limits_num_contexts_def]
+QED
+
+Theorem limits_num_contexts_revert[simp]:
+  limits_num_contexts n n revert
+Proof
+  rw[revert_def, limits_num_contexts_def]
+QED
+
+Theorem limits_num_contexts_set_return_data[simp]:
+  limits_num_contexts n n (set_return_data x)
+Proof
+  rw[set_return_data_def] >> tac
+QED
+
+Theorem limits_num_contexts_step_return[simp]:
+  limits_num_contexts n n (step_return x)
+Proof
+  rw[step_return_def] >> tac
+QED
+
+Theorem limits_num_contexts_step_invalid[simp]:
+  limits_num_contexts n n step_invalid
+Proof
+  rw[step_invalid_def] >> tac
+QED
+
+Theorem limits_num_contexts_add_to_delete[simp]:
+  limits_num_contexts n n (add_to_delete x)
+Proof
+  rw[add_to_delete_def, limits_num_contexts_def, return_def, all_accounts_def]
+QED
+
+Theorem limits_num_contexts_step_self_destruct[simp]:
+  limits_num_contexts n n step_self_destruct
+Proof
+  rw[step_self_destruct_def] \\ tac
+  \\ rw[update_accounts_def, set_accounts_def, limits_num_contexts_def,
+        return_def]
+QED
+
+Theorem limits_num_contexts_unuse_gas[simp]:
+  limits_num_contexts n n (unuse_gas x)
+Proof
+  rw[unuse_gas_def] >> tac
+QED
+
+Theorem limits_num_contexts_inc_pc[simp]:
+  limits_num_contexts n n inc_pc
+Proof
+  rw[inc_pc_def] >> tac
+QED
+
+Theorem limits_num_contexts_abort_unuse[simp]:
+  limits_num_contexts n n (abort_unuse x)
+Proof
+  rw[abort_unuse_def] >> tac
+QED
+
+Theorem limits_num_contexts_abort_call_value[simp]:
+  limits_num_contexts n n (abort_call_value x)
+Proof
+  rw[abort_call_value_def] >> tac
+QED
+
+Theorem limits_num_contexts_push_context[simp]:
+  limits_num_contexts n (SUC n) (push_context x)
+Proof
+  rw[push_context_def, limits_num_contexts_def, return_def, all_accounts_def]
+QED
+
+Theorem limits_num_contexts_update_accounts_transfer_value[simp]:
+  limits_num_contexts n n (update_accounts (transfer_value x y z))
+Proof
+  rw[update_accounts_def, limits_num_contexts_def, return_def,
+     all_accounts_def]
+QED
+
+Theorem limits_num_contexts_precompile_ecrecover[simp]:
+  limits_num_contexts n n precompile_ecrecover
+Proof
+  rw[precompile_ecrecover_def]
+QED
+
+Theorem limits_num_contexts_precompile_ecadd[simp]:
+  limits_num_contexts n n precompile_ecadd
+Proof
+  rw[precompile_ecadd_def]
+QED
+
+Theorem limits_num_contexts_precompile_ecmul[simp]:
+  limits_num_contexts n n precompile_ecmul
+Proof
+  rw[precompile_ecmul_def]
+QED
+
+Theorem limits_num_contexts_precompile_ecpairing[simp]:
+  limits_num_contexts n n precompile_ecpairing
+Proof
+  rw[precompile_ecpairing_def]
+QED
+
+Theorem limits_num_contexts_precompile_blake2f[simp]:
+  limits_num_contexts n n precompile_blake2f
+Proof
+  rw[precompile_blake2f_def]
+QED
+
+Theorem limits_num_contexts_precompile_modexp[simp]:
+  limits_num_contexts n n precompile_modexp
+Proof
+  rw[precompile_modexp_def] \\ tac
+QED
+
+Theorem limits_num_contexts_precompile_sha2_256[simp]:
+  limits_num_contexts n n precompile_sha2_256
+Proof
+  rw[precompile_sha2_256_def] \\ tac
+QED
+
+Theorem limits_num_contexts_precompile_identity[simp]:
+  limits_num_contexts n n precompile_identity
+Proof
+  rw[precompile_identity_def] \\ tac
+QED
+
+Theorem limits_num_contexts_precompile_ripemd_160[simp]:
+  limits_num_contexts n n precompile_ripemd_160
+Proof
+  rw[precompile_ripemd_160_def]
+QED
+
+Theorem limits_num_contexts_dispatch_precompiles[simp]:
+  limits_num_contexts n n (dispatch_precompiles x)
+Proof
+  rw[dispatch_precompiles_def]
+QED
+
+Theorem limits_num_contexts_mono:
+  limits_num_contexts n1 n2 f ∧ n0 ≤ n1 ∧ n2 ≤ n3 ⇒
+  limits_num_contexts n0 n3 f
+Proof
+  rw[limits_num_contexts_def]
+  \\ first_x_assum(qspec_then`s`mp_tac)
+  \\ rw[]
+QED
+
+Theorem limits_num_contexts_check:
+  (n > m ⇒ limits_num_contexts n n2 f) ∧
+  (∀n1. n1 ≤ (MIN (PRE n) m) ⇒ limits_num_contexts (SUC n1) n2 g)
+  ⇒
+  limits_num_contexts n n2 (do
+    sd <- get_num_contexts;
+    if sd > m then f else g
+  od)
+Proof
+  rw[limits_num_contexts_def, bind_def, ignore_bind_def,
+     get_num_contexts_def, return_def]
+  \\ rw[]
+  \\ first_x_assum irule
+  \\ Cases_on`n ≤ m` \\ gs[]
+  >- (qexists_tac`PRE n` \\ gs[])
+  \\ qexists_tac`m` \\ gs[]
+QED
+
+Theorem limits_num_contexts_step_call:
+  0 < n ∧ n ≤ context_limit + 2 ⇒
+  limits_num_contexts n (MIN (SUC n) (context_limit + 2)) (step_call x)
+Proof
+  strip_tac
+  \\ gs[step_call_def, UNCURRY]
+  \\ qpat_abbrev_tac`b1 = COND _ _ _`
+  \\ irule limits_num_contexts_bind \\ qexists_tac`n` \\ simp[] \\ gen_tac
+  \\ irule limits_num_contexts_bind \\ qexists_tac`n` \\ simp[] \\ gen_tac
+  \\ irule limits_num_contexts_bind \\ qexists_tac`n` \\ simp[] \\ gen_tac
+  \\ irule limits_num_contexts_bind \\ qexists_tac`n` \\ simp[] \\ gen_tac
+  \\ irule limits_num_contexts_bind \\ qexists_tac`n` \\ simp[] \\ gen_tac
+  \\ qpat_abbrev_tac`b2 = COND _ _ _`
+  \\ qpat_abbrev_tac`b3 = COND _ _ _`
+  \\ qpat_abbrev_tac`b4 = COND _ _ _`
+  \\ qpat_abbrev_tac`b5 = COND _ _ _`
+  \\ irule limits_num_contexts_ignore_bind \\ qexists_tac`n` \\ simp[]
+  \\ qpat_abbrev_tac`b6 = COND _ _ _`
+  \\ irule limits_num_contexts_ignore_bind \\ qexists_tac`n` \\ rw[Abbr`b5`]
+  \\ irule limits_num_contexts_ignore_bind \\ qexists_tac`n` \\ rw[]
+  \\ irule limits_num_contexts_bind \\ qexists_tac`n` \\ simp[] \\ gen_tac
+  \\ rw[]
+  >- ( irule limits_num_contexts_mono \\ qexistsl_tac[`n`,`n`] \\ simp[] )
+  \\ irule limits_num_contexts_ignore_bind \\ qexists_tac`n` \\ rw[]
+  \\ irule limits_num_contexts_check \\ simp[]
+  \\ reverse conj_tac
+  >- (
+    strip_tac
+    \\ irule limits_num_contexts_mono
+    \\ qexistsl_tac[`n`,`n`] \\ simp[] )
+  \\ gen_tac \\ strip_tac
+  \\ simp[proceed_call_def]
+  \\ irule limits_num_contexts_bind \\ qexists_tac`SUC n1` \\ simp[] \\ gen_tac
+  \\ irule limits_num_contexts_bind \\ qexists_tac`SUC n1` \\ simp[] \\ gen_tac
+  \\ irule limits_num_contexts_ignore_bind \\ qexists_tac`SUC n1` \\ simp[]
+  \\ reverse conj_tac >- rw[]
+  \\ irule limits_num_contexts_bind \\ qexists_tac`SUC n1` \\ simp[] \\ gen_tac
+  \\ irule limits_num_contexts_bind \\ qexists_tac`SUC n1` \\ simp[] \\ gen_tac
+  \\ irule limits_num_contexts_bind \\ qexists_tac`SUC n1` \\ simp[] \\ gen_tac
+  \\ irule limits_num_contexts_ignore_bind
+  \\ qexists_tac`SUC (SUC n1)`
+  \\ gs[]
+  \\ irule limits_num_contexts_mono
+  \\ qexistsl_tac[`n1 + 2`,`n1 + 2`] \\ rw[]
+QED
+
+Theorem limits_num_contexts_step_create:
+  0 < n ∧ n ≤ context_limit + 2 ⇒
+  limits_num_contexts n (MIN (SUC n) (context_limit + 2)) (step_create x)
+Proof
+  strip_tac
+  \\ gs[step_create_def]
+  \\ qpat_abbrev_tac`b1 = COND _ _ _`
+  \\ qpat_abbrev_tac`b2 = COND _ _ _`
+  \\ irule limits_num_contexts_bind \\ qexists_tac`n` \\ simp[] \\ gen_tac
+  \\ irule limits_num_contexts_bind \\ qexists_tac`n` \\ simp[] \\ gen_tac
+  \\ qpat_abbrev_tac`b3 = COND _ _ _`
+  \\ irule limits_num_contexts_ignore_bind \\ qexists_tac`n` \\ simp[]
+  \\ irule limits_num_contexts_ignore_bind \\ qexists_tac`n` \\ simp[]
+  \\ irule limits_num_contexts_bind \\ qexists_tac`n` \\ simp[] \\ gen_tac
+  \\ irule limits_num_contexts_bind \\ qexists_tac`n` \\ simp[] \\ gen_tac
+  \\ irule limits_num_contexts_bind \\ qexists_tac`n` \\ simp[] \\ gen_tac
+  \\ irule limits_num_contexts_ignore_bind \\ qexists_tac`n` \\ simp[]
+  \\ irule limits_num_contexts_ignore_bind \\ qexists_tac`n` \\ simp[]
+  \\ irule limits_num_contexts_bind \\ qexists_tac`n` \\ simp[] \\ gen_tac
+  \\ irule limits_num_contexts_ignore_bind \\ qexists_tac`n` \\ simp[]
+  \\ irule limits_num_contexts_ignore_bind \\ qexists_tac`n` \\ simp[]
+  \\ irule limits_num_contexts_ignore_bind \\ qexists_tac`n` \\ simp[]
+  \\ qpat_abbrev_tac`b4 = COND _ _ _`
+  \\ qmatch_goalsub_abbrev_tac`b5 ∨ _`
+  \\ Cases_on`b5` \\ gs[]
+  >- (
+    irule limits_num_contexts_mono \\ qexistsl_tac[`n`,`n`] \\ simp[]
+    \\ tac )
+  \\ qmatch_goalsub_abbrev_tac`b5 ∨ _`
+  \\ Cases_on`b5` \\ gs[]
+  >- (
+    irule limits_num_contexts_mono \\ qexistsl_tac[`n`,`n`] \\ simp[]
+    \\ tac )
+  \\ irule limits_num_contexts_check
+  \\ reverse conj_tac
+  >- (
+    strip_tac
+    \\ irule limits_num_contexts_mono
+    \\ qexistsl_tac[`n`,`n`] \\ simp[] )
+  \\ gen_tac \\ strip_tac
+  \\ simp[Abbr`b4`]
+  \\ `SUC n1 ≤ n` by gs[]
+  \\ `n ≤ MIN (SUC n) 1026` by gs[]
+  \\ IF_CASES_TAC
+  >- (
+    irule limits_num_contexts_mono
+    \\ qexistsl_tac[`n`,`n`] \\ simp[]
+    \\ rw[abort_create_exists_def]
+    \\ tac
+    \\ rw[limits_num_contexts_def, update_accounts_def, return_def])
+  \\ simp[proceed_create_def]
+  \\ qpat_abbrev_tac`b4 = COND _ _ _`
+  \\ irule limits_num_contexts_ignore_bind \\ qexists_tac`SUC n1` \\ simp[]
+  \\ reverse conj_tac >- rw[limits_num_contexts_def, update_accounts_def, return_def]
+  \\ irule limits_num_contexts_bind \\ qexists_tac`SUC n1` \\ simp[]
+  \\ gen_tac
+  \\ irule limits_num_contexts_ignore_bind \\ qexists_tac`SUC n1` \\ simp[]
+  \\ reverse conj_tac >- rw[limits_num_contexts_def, update_accounts_def, return_def]
+  \\ irule limits_num_contexts_mono
+  \\ qexistsl_tac[`SUC n1`,`SUC(SUC n1)`] \\ rw[]
+  \\ gs[]
+QED
+
+Theorem limits_num_contexts_step_inst:
+  n = context_limit + 2 ⇒
+  limits_num_contexts n n (step_inst op)
+Proof
+  Cases_on`op` \\ rw[step_inst_def]
+  >- (irule limits_num_contexts_ignore_bind_same \\ rw[])
+  \\ `MIN (SUC 1026) (context_limit + 2) = 1026` by rw[]
+  \\ `0 < 1026` by rw[]
+  \\ `1026 ≤ context_limit + 2` by rw[]
+  \\ drule_at Any limits_num_contexts_step_create \\ simp[]
+  \\ drule_at Any limits_num_contexts_step_call \\ simp[]
+QED
+
+Theorem limits_num_contexts_handle:
+  limits_num_contexts n n f ∧
+  (∀e. limits_num_contexts n n (g e))
+  ⇒
+  limits_num_contexts n n (handle f g)
+Proof
+  rw[handle_def, limits_num_contexts_def]
+  \\ CASE_TAC \\ gs[]
+  \\ CASE_TAC \\ gs[]
+  \\ metis_tac[SND]
+QED
+
+Theorem limits_num_contexts_get_output_to[simp]:
+  limits_num_contexts n n get_output_to
+Proof
+  rw[get_output_to_def] \\ tac
+QED
+
+Theorem limits_num_contexts_pop_and_incorporate_context[simp]:
+  limits_num_contexts n n (pop_and_incorporate_context x)
+Proof
+  rw[pop_and_incorporate_context_def]
+  \\ tac
+  \\ rw[bind_def, ignore_bind_def, pop_context_def, unuse_gas_def,
+        limits_num_contexts_def, fail_def, return_def, assert_def,
+        get_current_context_def, set_current_context_def, update_gas_refund_def,
+        push_logs_def, set_rollback_def]
+  \\ rw[] \\ rw[]
+  \\ Cases_on`s.contexts` \\ gs[]
+QED
+
+Theorem limits_num_contexts_reraise[simp]:
+  limits_num_contexts n n (reraise e)
+Proof
+  rw[reraise_def, limits_num_contexts_def]
+QED
+
+Theorem limits_num_contexts_step[simp]:
+  n = context_limit + 2 ⇒
+  limits_num_contexts n n step
+Proof
+  rw[step_def]
+  \\ irule limits_num_contexts_handle
+  \\ reverse conj_tac
+  >- (
+    irule limits_num_contexts_bind_same \\ rw[]
+    >- ( irule limits_num_contexts_step_inst \\ rw[] )
+    \\ CASE_TAC \\ rw[]
+    >- ( irule limits_num_contexts_step_inst \\ rw[] )
+    \\ irule limits_num_contexts_ignore_bind_same \\ rw[]
+    \\ TRY ( irule limits_num_contexts_step_inst \\ rw[] )
+    \\ rw[inc_pc_or_jump_def]
+    \\ tac
+    \\ CASE_TAC \\ rw[]
+    \\ tac)
+  \\ rw[handle_step_def]
+  \\ irule limits_num_contexts_handle
+  \\ conj_tac
+  >- (
+    simp[handle_exception_def] \\ gen_tac
+    \\ irule limits_num_contexts_ignore_bind_same
+    \\ reverse conj_tac
+    >- ( rw[] \\ tac )
+    \\ irule limits_num_contexts_bind_same \\ rw[]
+    \\ irule limits_num_contexts_bind_same \\ rw[]
+    \\ irule limits_num_contexts_bind_same \\ rw[]
+    \\ irule limits_num_contexts_ignore_bind_same \\ rw[]
+    \\ irule limits_num_contexts_ignore_bind_same \\ rw[]
+    \\ CASE_TAC \\ rw[] \\ CASE_TAC \\ rw[]
+    \\ tac )
+  \\ rw[handle_create_def]
+  \\ tac
+  \\ CASE_TAC \\ CASE_TAC \\ CASE_TAC \\ rw[]
+  \\ tac
+  >- rw[limits_num_contexts_def, update_accounts_def, return_def]
+  \\ rw[limits_num_contexts_def, assert_def, bind_def, update_accounts_def,
+        ignore_bind_def, return_def, reraise_def]
+QED
+
 Theorem step_preserves_wf_state:
   wf_state s ⇒ wf_state (SND (step s))
 Proof
   mp_tac decreases_gas_step
   \\ mp_tac preserves_wf_accounts_step
-  \\ rewrite_tac[decreases_gas_cred_def, preserves_wf_accounts_def]
+  \\ mp_tac (GEN_ALL limits_num_contexts_step)
+  \\ rewrite_tac[decreases_gas_cred_def, preserves_wf_accounts_def,
+                 limits_num_contexts_def]
   \\ rw[wf_state_def]
   >- ( first_x_assum(qspec_then`s`mp_tac) \\ rw[] )
-  >- cheat
+  >- ( `1026 = SUC 1025` by simp[] \\ metis_tac[LESS_EQ_IFF_LESS_SUC])
   >- ( first_x_assum(qspec_then`s`mp_tac) \\ simp[ok_state_def])
 QED
-*)
 
 val () = export_theory();
